
If this seems familiar its redundant with 
preceding section in mjm\_euv\_multi.tex.
However, the terms are grouped differently to show tri-diagonal
structure and detail the corner cases for small n.
I wrote "mjm\_math" to do a few polynomial manipulations
although it could probably be done in a variety of existing
things like mathematica or sympy. 

\begin{figure}[htb]
\centering

\cee{  X_0 + h$\nu$ -> X_1 }

\cee{  X_{i-1} + h$\nu$ -> X_i }

for i not equal zero or n,

\cee{  X_i ->[k] X_{i-1} }

\mjmeqn{\mjmdt{X_i}=-\phi X_i+\phi X_{i-1} + k X_{i+1}-k X_i 
= \phi X_{i-1} -(\phi + k )  X_i + k X_{i+1} }

otherwise with no decay from terminal state,

\mjmeqn{\mjmdt{X_n}=\phi X_{n-1} }
\mjmeqn{\mjmdt{X_{n-1}}=-(\phi+k) X_{n-1}+\phi X_{n-2}  }
\mjmeqn{\mjmdt{X_0}=-\phi X_0+ k X_{1} }


\caption{ With loss finite lifetime states but stable terminal state . }
\label{fig:leakynrepeat}
\end{figure}

\mjmtol{

wtf n=2,
%\mjmeqn{\mjmdt{X_2}=\phi X_{1} }
%\mjmeqn{\mjmdt{X_{1}}=-(\phi+k) X_{1}+\phi X_{0}  }
%\mjmeqn{\mjmdt{X_0}=-\phi X_0+ k X_{1} }


\mjmeqn{\mjmdtn{2}{X_2}=\phi \mjmdt{X_{1}} }
\mjmeqn{\mjmdtn{2}{X_2}=\left( -(\phi+k)\phi X_{1}+\phi^2 X_{0}   \right) } 
\mjmeqn{\mjmdtn{2}{X_2}=\left( -(\phi+k)\mjmdt{X_{2}}+\phi^2 X_{0}   \right) } 
\mjmeqn{\mjmdtn{2}{X_2}+(\phi+k)\mjmdt{X_{2}}= \phi^2 X_{0}    } 
\mjmeqn{\mjmdtn{3}{X_2}+(\phi+k)\mjmdtn{2}{X_{2}}= \phi^2 \mjmdt{X_{0}  }  } 
\mjmeqn{\mjmdtn{3}{X_2}+(\phi+k)\mjmdtn{2}{X_{2}}
= \phi^2 \left( -\phi X_0+ k X_{1} \right)  }  

\mjmeqn{\mjmdtn{3}{X_2}+(\phi+k)\mjmdtn{2}{X_{2}}
= -\phi^3 X_0+ k\phi \mjmdt{ X_{2} }  }  

\mjmeqn{\mjmdtn{3}{X_2}+(\phi+k)\mjmdtn{2}{X_{2}}
- k\phi \mjmdt{X_{2}}  = -\phi^3 X_0 }  

\mjmeqn{\mjmdtn{3}{X_2}+(\phi+k)\mjmdtn{2}{X_{2}}
- k\phi \mjmdt{X_{2}}  = 
-\phi  \left( \mjmdtn{2}{X_2}+(\phi+k)\mjmdt{X_{2}} \right)
}  
\mjmeqn{\mjmdtn{3}{X_2}+(2*\phi+k)\mjmdtn{2}{X_{2}}
+\phi^2 \mjmdt{X_{2}}  = 0
}  
\mjmeqn{ r(r^2+(2\phi+k)r+\phi^2) =0 }

\mjmeqn{ b^2=4\phi^2+k^2+4k\phi  }
\mjmeqn{ b^2-4ac=k^2+4k\phi  }
\mjmeqn{ r=-\phi-\frac{k}{2} \pm \sqrt{k(k+4\phi)}   }

} % mjtol 


\mjmtol{

 n=3,
\mjmeqn{\mjmdt{X_3}=\phi X_{2} }
\mjmeqn{\mjmdt{X_{2}}=-(\phi+k) X_{2}+\phi X_{1}  }
\mjmeqn{\mjmdt{X_{1}}=-(\phi+k) X_{1}+\phi X_{0}-k X_{2}  }
\mjmeqn{\mjmdt{X_0}=-\phi X_0+ k X_{1} }


\mjmeqn{\mjmdtn{2}{X_3}=\phi \mjmdt{X_{2}} }
\mjmeqn{\mjmdtn{2}{X_3}=\left( -(\phi+k)\phi X_{2}+\phi^2 X_{1}   \right) } 
\mjmeqn{\mjmdtn{2}{X_2}=\left( -(\phi+k)\mjmdt{X_{3}}+\phi^2 X_{1}   \right) } 
\mjmeqn{\mjmdtn{2}{X_3}+(\phi+k)\mjmdt{X_{3}}= \phi^2 X_{1}    } 


\mjmeqn{\mjmdtn{3}{X_3}+(\phi+k)\mjmdtn{2}{X_{3}}= \phi^2 \mjmdt{X_{1}}    } 

\mjmeqn{\mjmdtn{3}{X_3}+(\phi+k)\mjmdtn{2}{X_{3}}= \phi^2 
%\mjmdt{X_{1}}    
\left( -(\phi+k) X_{1}+\phi X_{0}-k X_{2}  \right)
} 

\mjmeqn{\mjmdtn{3}{X_3}+(\phi+k)\mjmdtn{2}{X_{3}}=  
%-\phi^2(\phi+k) X_{1}
-(\phi+k)(\mjmdtn{2}{X_3}+(\phi+k)\mjmdt{X_{3}})  
+\phi^3 X_{0}
%-k\phi^2 X_{2}  
-k\phi \mjmdt{X_{3} } 
} 

\mjmeqn{\mjmdtn{3}{X_3}+2(\phi+k)\mjmdtn{2}{X_{3}}
+((\phi+k)^2+k\phi)\mjmdt{X_{3}})  
=  \phi^3 X_{0}
} 

%\mjmeqn{\mjmdt{X_0}=-\phi X_0+ k X_{1} }
\mjmeqn{\mjmdtn{4}{X_3}+2(\phi+k)\mjmdtn{3}{X_{3}}
+((\phi+k)^2+k\phi)\mjmdtn{2}{X_{3}})  
=   
 -\phi^4 X_0
+ k\phi^3 X_{1} 
} 



} % ssck n=3
\mjmtol{ n==3 part 2

repeat,

\mjmeqn{\mjmdtn{4}{X_3}+2(\phi+k)\mjmdtn{3}{X_{3}}
+((\phi+k)^2+k\phi)\mjmdtn{2}{X_{3}})  
=   
 -\phi^4 X_0
+ k\phi^3 X_{1} 
} 

use identities,
\mjmeqn{\mjmdtn{3}{X_3}+2(\phi+k)\mjmdtn{2}{X_{3}}
+((\phi+k)^2+k\phi)\mjmdt{X_{3}})  
=  \phi^3 X_{0}
} 
\mjmeqn{\mjmdtn{3}{X_3}+(\phi+k)\mjmdtn{2}{X_{3}}= \phi^2 \mjmdt{X_{1}}    } 
\mjmeqn{\mjmdtn{2}{X_3}+(\phi+k)\mjmdt{X_{3}}= \phi^2 X_{1}    } 

\mjmeqn{\mjmdtn{4}{X_3}+2(\phi+k)\mjmdtn{3}{X_{3}}
+((\phi+k)^2+k\phi)\mjmdtn{2}{X_{3}})  
=   
% -\phi^4 X_0
-\phi\mjmdtn{3}{X_3} -\phi 2(\phi+k)\mjmdtn{2}{X_{3}}
-\phi((\phi+k)^2+k\phi)\mjmdt{X_{3}})  
%+ k\phi^3 X_{1} 
+k\phi\mjmdtn{2}{X_3}+k\phi(\phi+k)\mjmdt{X_{3}} 
} 

\mjmeqn{\mjmdtn{4}{X_3}
+(3\phi+2k)\mjmdtn{3}{X_{3}}
+((\phi+k)^2+2k\phi+2\phi^2)\mjmdtn{2}{X_{3}}  
+\phi((\phi+k)^2-k*k)\mjmdt{X_{3}}  
=  0 
% -\phi^4 X_0
%+ k\phi^3 X_{1} 
} 


\mjmeqn{\mjmdtn{4}{X_3}
+(3\phi+2k)\mjmdtn{3}{X_{3}}
%+((\phi+k)^2+2k\phi+2\phi^2)\mjmdtn{2}{X_{3}}  
+(k^2+4k\phi +3\phi^2)\mjmdtn{2}{X_{3}}  
%+\phi((\phi+k)^2-k*k)\mjmdt{X_{3}}  
+(\phi^3+2k\phi^2 )\mjmdt{X_{3}}  
=  0 
% -\phi^4 X_0
%+ k\phi^3 X_{1} 
} 




} % n==3 part2




The characteristic equation then is,

\mjmeqn{\mjmdtn{2}{X_n}=\phi \mjmdt{X_{n-1}} }
\mjmeqn{\mjmdtn{2}{X_n}=
  \phi  \left( -(\phi+k) \mjmdt{X_{n-1}}+\phi \mjmdt{X_{n-2}}   \right) }

\mjmeqn{\mjmdtn{2}{X_n}=
  \phi  \left( -(\phi+k)\mjmdt{X_n}+\phi \mjmdt{X_{n-2}} \right) }

\mjmeqn{\mjmdtn{2}{X_n}=
   -(\phi+k)\phi\mjmdt{X_n}+\phi^2 \mjmdt{X_{n-2}}  }

\mjmeqn{\mjmdtn{2}{X_n}+ (\phi+k)\phi \mjmdt{X_n}
=\phi^2 \mjmdt{X_{n-2}}  }

For n=2, 
%\mjmeqn{\mjmdtn{2}{X_2}+ (\phi+k) \mjmdt{X_2} =\phi^2\left( -\phi X_0+ k X_{1} \right) =-\phi^3 X_0+ k\phi^2 \mjmdt{X_{2}} }
%\mjmeqn{\mjmdtn{2}{X_2}+ (\phi+k) \mjmdt{X_2} =\phi^2\left( -\phi X_0+ k X_{1} \right) =-\phi^3 X_0+ k \phi X_{1} }


\mjmeqn{\mjmdtn{2}{X_2}+ (\phi+k)\phi \mjmdt{X_2}
=\phi^2\left( -\phi X_0+ k X_{1} \right)
=-\phi^3 X_0+ k\phi \mjmdt{X_{2}} 
}


\mjmeqn{\mjmdtn{2}{X_2}+\phi^2\mjmdt{X_2} =-\phi^3 X_0 }

\mjmeqn{\mjmdtn{3}{X_2}+ \phi^2  \mjmdtn{2}{X_2} =-\phi^3 \mjmdt{X_0}
= \phi^4 X_0 - \phi^3 k X_1
 }
\mjmeqn{\mjmdtn{3}{X_2}+ \phi^2 \mjmdtn{2}{X_2} =-\phi^3 \mjmdt{X_0}
= 
% \phi^4 X_0 
- \phi \mjmdtn{2}{X_2} - \phi^3\mjmdt{X_2} 
- \phi^3 k X_1
 }

\mjmeqn{\mjmdtn{3}{X_2}+ (\phi^2+\phi ) \mjmdtn{2}{X_2} 
+ \phi^3 \mjmdt{X_2} 
=- \phi^3 k X_1 = -\phi^2 k \mjmdt{X_2}
 }

%%%%%%%%%%%%%%%%%%%%%%%%%%%%%%%%%%%%%%


\mjmeqn{\mjmdtn{3}{X_2}+ (\phi^2+\phi ) \mjmdtn{2}{X_2} 
+  ( \phi^3 +\phi^2 k) \mjmdt{X_2} =0 
 }


\mjmeqn{ r(r^2+r(\phi+\phi^2)+\phi^2(\phi+k) ) =0 }

\mjmeqn{ b^2=  \phi^2(1+2\phi+\phi^2)  }
\mjmeqn{ b^2-4ac=  \phi^2(1+2\phi+\phi^2)-4*\phi^2(\phi+k)   }



%\mjmeqn{\mjmdtn{3}{X_2}+ (\phi+k-k\phi ) \mjmdtn{2}{X_2} =-\phi^3 \mjmdt{X_0} =-\phi \left( \mjmdtn{2}{X_2}+ (\phi+k) \mjmdt{X_1} \right) }


%\mjmeqn{\mjmdtn{3}{X_2}+ (2*\phi+k-k\phi ) \mjmdtn{2}{X_2} =-  (\phi+k) \mjmdtn{2}{X_2} }





